hmacdrbg/drbg_protocol_proofs.v
@@ -463,7 +463,6 @@ Proof.
   { forward. entailer!. }
   { forward. (*red in WFI; simpl in WFI.*) entailer!. simpl.
       unfold Int.ltu; simpl.
-      rewrite add_repr.
       rewrite Int.unsigned_repr. 2: rewrite int_max_unsigned_eq; omega.
       rewrite Int.unsigned_repr_eq, Zmod_small.
       + destruct (zlt 384 (entropy_len + (Zlength contents))); simpl; try reflexivity.
