progs/verif_switch.v
@@ -10,7 +10,7 @@ Definition twice_spec :=
   DECLARE _twice
     WITH n : Z
     PRE [ _n OF tint ]
-      PROP  (0 <= n+n <= Int.max_unsigned)
+      PROP  (0 <= n+n <= Int.max_signed)
       LOCAL (temp _n (Vint (Int.repr n)))
       SEP ()
     POST [ tint ]
@@ -24,6 +24,7 @@ Lemma body_twice: semax_body Vprog Gprog f_twice twice_spec.
 Proof.
 start_function.
 forward_if (PROP() LOCAL(temp _n (Vint (Int.repr (n+n)))) SEP()).
+ repable_signed.
 repeat forward; entailer!.
 repeat forward; entailer!.
 repeat forward; entailer!.
